util/meta/tactic/monotonicity/default.lean
@@ -1,0 +1,3 @@
+
+import util.meta.tactic.monotonicity.predicate
+import util.meta.tactic.monotonicity.function
