util/meta/tactic/monotonicity/function.lean
@@ -1,11 +1,9 @@
 
 import data.dlist
 
-import util.logic
-import util.data.traversable
-import util.control.monad
-
+import util.algebra.group
 import util.data.list
+import util.data.traversable
 
 variables {a b c p : Prop}
 
@@ -17,131 +15,6 @@ open tactic
 
 local postfix `?`:9001 := optional
 local postfix *:9001 := many
-
-meta def match_exists : expr → tactic (name × expr × expr)
- | `(@Exists _ %%e) := return (expr.binding_name e
-                           ,expr.binding_domain e
-                           ,expr.binding_body e)
- | _ := fail "expecting an existential"
-
-meta def match_forall : expr → tactic (name × expr × expr)
- | (expr.pi n _ d b) := return (n,d,b)
- | e := fail $ format! "expecting a universal {e}"
-
-/-- for goals of the form `f x → f x'` for certain monotonic or antimonotonic f,
-    bring the context of `x` into the assumptions.
-    Possible f are
-      (∃ x, _)
-      (∀ x, _)
-      →, ∧, ∨, ¬
-    TODO: add monotonicity type class
--/
-meta def intro_mono (id : parse ident_ ?) : tactic unit :=
-do g ← target >>= instantiate_mvars,
-   match g with
-    | `( (∃ x : %%t₀, %%e₀) → (∃ x : %%t₁, %%e₁) ) :=
-      do (is_def_eq t₀ t₁
-            <|> fail (format! "type of bound variables don't match: {t₀} ≠ {t₁}")),
-         `[apply exists_imp_exists],
-         intro id
-    | `( (∀ x : %%t₀, %%e₀) → (∀ x : %%t₁, %%e₁) ) :=
-        (do is_def_eq t₀ t₁,
-            `[apply forall_imp_forall _],
-            intro id)
-    <|> (do (guard (¬ e₀.has_var ∧ ¬ e₁.has_var)
-                   <|> fail (format! "type of bound variables don't match: {t₀} ≠ {t₁}")),
-            is_def_eq e₀ e₁,
-            p ← to_expr ``(%%t₁ → %%t₀),
-            assert `h p,
-            swap,
-            `[intros h₀ h₁, apply h₀, apply h h₁])
-    | `( (%%t₀ ∧ %%e₀) → (%%t₁ ∧ %%e₁) ) :=
-        (do is_def_eq t₀ t₁,
-            `[apply and.mono_right],
-            intro id)
-    <|> (do is_def_eq e₀ e₁,
-            `[apply and.mono_left],
-            intro id)
-    | `( (%%t₀ ∨ %%e₀) → (%%t₁ ∨ %%e₁) ) :=
-        (do is_def_eq t₀ t₁,
-            `[apply classical.or.mono_right],
-            intro id)
-    <|> (do is_def_eq e₀ e₁,
-            `[apply classical.or.mono_left],
-            intro id)
-    | `( (¬ %%e₀) → (¬ %%e₁) ) :=
-        (`[apply mt])
-    | _ := fail "cannot apply monotonicity rules to goal"
-   end
-
-meta def intros_mono_dep : tactic unit :=
-do g ← target,
-   match g with
-    | `(%%e₀ → %%e₁) :=
-        (do (n₀,t₀,e₀) ← match_exists e₀,
-            (n₁,t₁,e₁) ← match_exists e₁,
-            if e₀.has_var_idx 0 then intro_mono (some n₀) >> intros_mono_dep
-            else if e₁.has_var_idx 0 then intro_mono (some n₁) >> intros_mono_dep
-            else return ())
-    <|> (do (n₀,t₀,e₀) ← match_forall e₀,
-            (n₁,t₁,e₁) ← match_forall e₁,
-            if e₀.has_var_idx 0 then intro_mono (some n₀) >> intros_mono_dep
-            else if e₁.has_var_idx 0 then intro_mono (some n₁) >> intros_mono_dep
-            else return ())
-    <|> (do expr.is_not e₀,
-            expr.is_not e₁,
-            intro_mono none >> intros_mono_dep)
-    <|> return ()
-    | _ := fail "expecting an implication"
-   end
-
-meta def introv_mono : parse ident_ * → tactic unit
- | [] := intros_mono_dep
- | (x::xs) := intros_mono_dep >> intro_mono (some x) >> introv_mono xs
-
-meta def intros_mono : parse ident_ * → tactic unit
- | [] := repeat (intro_mono none)
- | xs := mmap' (intro_mono ∘ some) xs
-
-example {α β : Type} (p q : α → β → Prop) (r : α → Prop) (s : β → Prop)
-  (h : ∀ x y, r x → ¬ s y → q x y → p x y)
-: (∃ x, ∀ y, r x ∧ (¬ p x y ∨ s y))
-→ (∃ i, ∀ j, r i ∧ (¬ q i j ∨ s j)) :=
-begin
-  intro_mono k,
-  intro_mono z,
-  intro_mono i,
-  intro_mono j,
-  intro_mono ,
-  apply h ; assumption
-end
-
-example {α β : Type} (p q : α → β → Prop) (r : α → Prop) (s : β → Prop)
-  (h : ∀ x y, r x → ¬ s y → q x y → p x y)
-: (∃ x, ∀ y, r x ∧ (¬ p x y ∨ s y))
-→ (∃ i, ∀ j, r i ∧ (¬ q i j ∨ s j)) :=
-begin
-  intros_mono,
-  apply h ; assumption
-end
-
-example {α β : Type} (p q : α → β → Prop) (r : α → Prop) (s : β → Prop)
-  (h : ∀ x y, r x → ¬ s y → q x y → p x y)
-: (∃ x, ∀ y, r x ∧ (¬ p x y ∨ s y))
-→ (∃ i, ∀ j, r i ∧ (¬ q i j ∨ s j)) :=
-begin
-  intros_mono,
-  apply h ; assumption,
-end
-
-example {α β : Type} (p : α → β → Prop) (r : α → Prop) (s : β → Prop)
-  (h : ∀ x y, r x → ¬ r x → p x y → r x)
-: (∃ x, ∀ y : β, r x ∧ (¬ r x ∨ r x))
-→ (∃ i, ∀ j, r i ∧ (¬ p i j ∨ r i)) :=
-begin
-  introv_mono h₀ h₁,
-  apply h ; assumption,
-end
 
 meta inductive mono_function (elab : bool := tt)
  | non_assoc : expr elab → list (expr elab) → list (expr elab) → mono_function
@@ -322,6 +195,7 @@ meta def check_ac : expr → tactic (bool × bool × option (expr × expr) × ex
 
 run_cmd
 do x ← to_expr ``(7 + 3 : ℕ) >>= check_ac,
+   trace x,
    x ← pp x.2.2.1,
    guard $ x.to_string = "(some (add_monoid_to_is_left_id, 0))"
 
